fstar-helpers/minicore/src/abstractions/funarr.rs
@@ -3,7 +3,7 @@
 open FStar.Tactics
 
 let ${_pointwise_apply_mk_term} #t
-  (max: nat)
+  (max: nat{max > 0})
   (f: (n:nat {n < max}) -> t)
   : Tac unit
   = let rec brs (n:nat): Tac _ = 
@@ -13,7 +13,7 @@ let ${_pointwise_apply_mk_term} #t
       ::( match n with | 0 -> [] | _ -> brs (n - 1))
     in
     let bd = fresh_binder_named "i" (quote (m: nat {m < max})) in
-    let t = mk_abs [bd] (Tv_Match bd None (brs max)) in
+    let t = mk_abs [bd] (Tv_Match bd None (brs (max - 1))) in
     exact t"#
 )]
 pub fn _pointwise_apply_mk_term() {}
