libcrux-ml-dsa/src/simd/avx2/encoding/commitment.rs
@@ -2,6 +2,37 @@ use libcrux_intrinsics::avx2::*;
 
 use minicore::abstractions::{bit::Bit, bitvec::BitVec};
 
+// #[hax_lib::fstar::before(
+//     r#"[@@(FStar.Tactics.postprocess_with ${BitVec::<128>::postprocess_rewrite})]"#
+// )]
+// fn serialize_6(simd_unit: &Vec256) -> (Vec128, Vec128) {
+//     let adjacent_2_combined =
+//         mm256_sllv_epi32(*simd_unit, mm256_set_epi32(0, 26, 0, 26, 0, 26, 0, 26));
+//     let adjacent_2_combined = mm256_srli_epi64::<26>(adjacent_2_combined);
+
+//     let adjacent_3_combined = mm256_shuffle_epi8(
+//         adjacent_2_combined,
+//         mm256_set_epi8(
+//             -1, -1, -1, -1, -1, -1, -1, -1, -1, -1, -1, -1, 9, 8, 1, 0, -1, -1, -1, -1, -1, -1, -1,
+//             -1, -1, -1, -1, -1, 9, 8, 1, 0,
+//         ),
+//     );
+
+//     let adjacent_3_combined = mm256_mullo_epi16(
+//         adjacent_3_combined,
+//         mm256_set_epi16(1, 1, 1, 1, 1, 1, 1, 1 << 4, 1, 1, 1, 1, 1, 1, 1, 1 << 4),
+//     );
+//     let adjacent_3_combined =
+//         mm256_srlv_epi32(adjacent_3_combined, mm256_set_epi32(0, 0, 0, 4, 0, 0, 0, 4));
+
+//     // We now have 24 bits starting at position 0 in the lower 128-bit lane, ...
+//     let lower_3 = mm256_castsi256_si128(adjacent_3_combined);
+
+//     // and 24 bits starting at position 0 in the upper 128-bit lane.
+//     let upper_3 = mm256_extracti128_si256::<1>(adjacent_3_combined);
+//     (lower_3, upper_3)
+// }
+
 #[hax_lib::ensures(|r| {
     use hax_lib::*;
     let r = BitVec::<128>::from(r);
@@ -12,52 +43,33 @@ use minicore::abstractions::{bit::Bit, bitvec::BitVec};
 })]
 #[inline(always)]
 fn serialize_4(simd_unit: &Vec256) -> Vec128 {
-    #[hax_lib::fstar::before(r#"
-    [@@FStar.Tactics.V2.(postprocess_with (fun () -> 
-            let done = alloc false in
-            ctrl_rewrite TopDown (fun _ -> if read done then (false, Skip) else (true, Continue))
-                                 (fun _ -> (fun () -> apply_lemma_rw (`${BitVec::<128>::rewrite_pointwise}); write done true)
-                                           `or_else` trefl);
-            let crate = match cur_module () with | crate::_ -> crate | _ -> fail "Empty module name" in
-            norm [primops; iota; delta_namespace ["Core"; crate; "Libcrux_intrinsics"; "Minicore"; "FStar.FunctionalExtensionality"; "Rust_primitives"]; zeta_full];
-            compute ();
-            norm [primops; iota; delta; zeta_full];
-            trefl ()
-            ))]
-    "#)]
+    #[hax_lib::fstar::before(
+        r#"[@@(FStar.Tactics.postprocess_with ${BitVec::<128>::postprocess_rewrite})]"#
+    )]
     #[inline(always)]
-    fn aux(simd_unit: Vec256) -> Vec128 {
-        let adjacent_2_combined = mm256_sllv_epi32_u32(simd_unit, 0, 28, 0, 28, 0, 28, 0, 28);
-        let x = adjacent_2_combined;
+    fn aux(simd_unit: &Vec256) -> Vec128 {
+        let adjacent_2_combined =
+            mm256_sllv_epi32(*simd_unit, mm256_set_epi32(0, 28, 0, 28, 0, 28, 0, 28));
         let adjacent_2_combined = mm256_srli_epi64::<28>(adjacent_2_combined);
 
-        let adjacent_4_combined =
-            mm256_permutevar8x32_epi32_u32(adjacent_2_combined, 0, 0, 0, 0, 6, 2, 4, 0);
+        let adjacent_4_combined = mm256_permutevar8x32_epi32(
+            adjacent_2_combined,
+            mm256_set_epi32(0, 0, 0, 0, 6, 2, 4, 0),
+        );
         let adjacent_4_combined = mm256_castsi256_si128(adjacent_4_combined);
-        mm_shuffle_epi8_u8(
+        let adjacent_4_combined = mm_shuffle_epi8(
             adjacent_4_combined,
-            0xF0,
-            0xF0,
-            0xF0,
-            0xF0,
-            0xF0,
-            0xF0,
-            0xF0,
-            0xF0,
-            0xF0,
-            0xF0,
-            0xF0,
-            0xF0,
-            12,
-            4,
-            8,
-            0,
-        )
+            mm_set_epi8(
+                0xF0, 0xF0, 0xF0, 0xF0, 0xF0, 0xF0, 0xF0, 0xF0, 0xF0, 0xF0, 0xF0, 0xF0, 12, 4, 8, 0,
+            ),
+        );
+        adjacent_4_combined
     }
-    aux(*simd_unit)
+    aux(simd_unit)
 }
 
 #[inline(always)]
+#[hax_lib::requires(out.len() == 4 || out.len() == 6)]
 pub(in crate::simd::avx2) fn serialize(simd_unit: &Vec256, out: &mut [u8]) {
     let mut serialized = [0u8; 19];
 
