fstar-helpers/minicore/proofs/fstar/extraction/Minicore.Arch.X86.fst
@@ -9,6 +9,42 @@ let _ =
   let open Minicore.Abstractions.Bitvec in
   ()
 
+assume
+val e_mm256_set_epi32':
+    e0: i32 ->
+    e1: i32 ->
+    e2: i32 ->
+    e3: i32 ->
+    e4: i32 ->
+    e5: i32 ->
+    e6: i32 ->
+    e7: i32
+  -> Minicore.Abstractions.Bitvec.t_BitVec (mk_u64 256)
+
+let e_mm256_set_epi32 = e_mm256_set_epi32'
+
+assume
+val e_mm_set_epi8':
+    e15: i8 ->
+    e14: i8 ->
+    e13: i8 ->
+    e12: i8 ->
+    e11: i8 ->
+    e10: i8 ->
+    e9: i8 ->
+    e8: i8 ->
+    e7: i8 ->
+    e6: i8 ->
+    e5: i8 ->
+    e4: i8 ->
+    e3: i8 ->
+    e2: i8 ->
+    e1: i8 ->
+    e0: i8
+  -> Minicore.Abstractions.Bitvec.t_BitVec (mk_u64 128)
+
+let e_mm_set_epi8 = e_mm_set_epi8'
+
 let e_mm256_slli_epi16
       (v_SHIFT_BY: i32)
       (vector: Minicore.Abstractions.Bitvec.t_BitVec (mk_u64 256))
@@ -39,9 +75,146 @@ let e_mm256_srli_epi64
         then vector.[ i +! shift <: u64 ]
         else Minicore.Abstractions.Bit.Bit_Zero <: Minicore.Abstractions.Bit.t_Bit)
 
+assume
+val e_mm256_sllv_epi32':
+    vector: Minicore.Abstractions.Bitvec.t_BitVec (mk_u64 256) ->
+    counts: Minicore.Abstractions.Bitvec.t_BitVec (mk_u64 256)
+  -> Minicore.Abstractions.Bitvec.t_BitVec (mk_u64 256)
+
+let e_mm256_sllv_epi32 = e_mm256_sllv_epi32'
+
+assume
+val e_mm256_permutevar8x32_epi32':
+    a: Minicore.Abstractions.Bitvec.t_BitVec (mk_u64 256) ->
+    b: Minicore.Abstractions.Bitvec.t_BitVec (mk_u64 256)
+  -> Minicore.Abstractions.Bitvec.t_BitVec (mk_u64 256)
+
+let e_mm256_permutevar8x32_epi32 = e_mm256_permutevar8x32_epi32'
+
 let e_mm256_castsi256_si128 (vector: Minicore.Abstractions.Bitvec.t_BitVec (mk_u64 256))
     : Minicore.Abstractions.Bitvec.t_BitVec (mk_u64 128) =
   Minicore.Abstractions.Bitvec.impl_9__from_fn (mk_u64 128)
     (fun i ->
         let i:u64 = i in
         vector.[ i ] <: Minicore.Abstractions.Bit.t_Bit)
+
+assume
+val e_mm_shuffle_epi8':
+    vector: Minicore.Abstractions.Bitvec.t_BitVec (mk_u64 128) ->
+    indexes: Minicore.Abstractions.Bitvec.t_BitVec (mk_u64 128)
+  -> Minicore.Abstractions.Bitvec.t_BitVec (mk_u64 128)
+
+let e_mm_shuffle_epi8 = e_mm_shuffle_epi8'
+
+/// Rewrite lemmas
+let e_: Prims.unit = ()
+
+[@@ Minicore.Abstractions.Bitvec.v_REWRITE_RULE ]
+
+assume
+val e___e_rw_mm256_sllv_epi32':
+    vector: Minicore.Abstractions.Bitvec.t_BitVec (mk_u64 256) ->
+    b7: i32 ->
+    b6: i32 ->
+    b5: i32 ->
+    b4: i32 ->
+    b3: i32 ->
+    b2: i32 ->
+    b1: i32 ->
+    b0: i32
+  -> Lemma
+    (ensures
+      (e_mm256_sllv_epi32 vector
+          (e_mm256_set_epi32 b7 b6 b5 b4 b3 b2 b1 b0
+            <:
+            Minicore.Abstractions.Bitvec.t_BitVec (mk_u64 256))
+        <:
+        Minicore.Abstractions.Bitvec.t_BitVec (mk_u64 256)) ==
+      (Minicore.Arch.X86.Extra.mm256_sllv_epi32_u32 vector
+          (cast (b7 <: i32) <: u32)
+          (cast (b6 <: i32) <: u32)
+          (cast (b5 <: i32) <: u32)
+          (cast (b4 <: i32) <: u32)
+          (cast (b3 <: i32) <: u32)
+          (cast (b2 <: i32) <: u32)
+          (cast (b1 <: i32) <: u32)
+          (cast (b0 <: i32) <: u32)
+        <:
+        Minicore.Abstractions.Bitvec.t_BitVec (mk_u64 256)))
+
+let e___e_rw_mm256_sllv_epi32 = e___e_rw_mm256_sllv_epi32'
+
+[@@ Minicore.Abstractions.Bitvec.v_REWRITE_RULE ]
+
+assume
+val e___e_rw_mm256_permutevar8x32_epi32':
+    vector: Minicore.Abstractions.Bitvec.t_BitVec (mk_u64 256) ->
+    b7: i32 ->
+    b6: i32 ->
+    b5: i32 ->
+    b4: i32 ->
+    b3: i32 ->
+    b2: i32 ->
+    b1: i32 ->
+    b0: i32
+  -> Lemma
+    (ensures
+      (e_mm256_permutevar8x32_epi32 vector
+          (e_mm256_set_epi32 b7 b6 b5 b4 b3 b2 b1 b0
+            <:
+            Minicore.Abstractions.Bitvec.t_BitVec (mk_u64 256))
+        <:
+        Minicore.Abstractions.Bitvec.t_BitVec (mk_u64 256)) ==
+      (Minicore.Arch.X86.Extra.mm256_permutevar8x32_epi32_u32 vector
+          (cast (b7 <: i32) <: u32)
+          (cast (b6 <: i32) <: u32)
+          (cast (b5 <: i32) <: u32)
+          (cast (b4 <: i32) <: u32)
+          (cast (b3 <: i32) <: u32)
+          (cast (b2 <: i32) <: u32)
+          (cast (b1 <: i32) <: u32)
+          (cast (b0 <: i32) <: u32)
+        <:
+        Minicore.Abstractions.Bitvec.t_BitVec (mk_u64 256)))
+
+let e___e_rw_mm256_permutevar8x32_epi32 = e___e_rw_mm256_permutevar8x32_epi32'
+
+[@@ Minicore.Abstractions.Bitvec.v_REWRITE_RULE ]
+
+assume
+val e___e_rw_mm_shuffle_epi8':
+    vector: Minicore.Abstractions.Bitvec.t_BitVec (mk_u64 128) ->
+    e15: i8 ->
+    e14: i8 ->
+    e13: i8 ->
+    e12: i8 ->
+    e11: i8 ->
+    e10: i8 ->
+    e9: i8 ->
+    e8: i8 ->
+    e7: i8 ->
+    e6: i8 ->
+    e5: i8 ->
+    e4: i8 ->
+    e3: i8 ->
+    e2: i8 ->
+    e1: i8 ->
+    e0: i8
+  -> Lemma
+    (ensures
+      (e_mm_shuffle_epi8 vector
+          (e_mm_set_epi8 e15 e14 e13 e12 e11 e10 e9 e8 e7 e6 e5 e4 e3 e2 e1 e0
+            <:
+            Minicore.Abstractions.Bitvec.t_BitVec (mk_u64 128))
+        <:
+        Minicore.Abstractions.Bitvec.t_BitVec (mk_u64 128)) ==
+      (Minicore.Arch.X86.Extra.mm_shuffle_epi8_u8 vector (cast (e15 <: i8) <: u8)
+          (cast (e14 <: i8) <: u8) (cast (e13 <: i8) <: u8) (cast (e12 <: i8) <: u8)
+          (cast (e11 <: i8) <: u8) (cast (e10 <: i8) <: u8) (cast (e9 <: i8) <: u8)
+          (cast (e8 <: i8) <: u8) (cast (e7 <: i8) <: u8) (cast (e6 <: i8) <: u8)
+          (cast (e5 <: i8) <: u8) (cast (e4 <: i8) <: u8) (cast (e3 <: i8) <: u8)
+          (cast (e2 <: i8) <: u8) (cast (e1 <: i8) <: u8) (cast (e0 <: i8) <: u8)
+        <:
+        Minicore.Abstractions.Bitvec.t_BitVec (mk_u64 128)))
+
+let e___e_rw_mm_shuffle_epi8 = e___e_rw_mm_shuffle_epi8'
