libcrux-intrinsics/proofs/fstar/extraction/Libcrux_intrinsics.Avx2_extract.fst
@@ -3,278 +3,234 @@ module Libcrux_intrinsics.Avx2_extract
 open Core
 open FStar.Mul
 
-let mm256_storeu_si256_u8
-      (output: t_Slice u8)
-      (vector: Minicore.Abstractions.Bitvec.t_BitVec (mk_u64 256))
-    : t_Slice u8 =
-  let _:Prims.unit =
-    if true
-    then
-      let _:Prims.unit =
-        match Core.Slice.impl__len #u8 output, mk_usize 32 <: (usize & usize) with
-        | left_val, right_val -> Hax_lib.v_assert (left_val =. right_val <: bool)
-      in
-      ()
-  in
-  let _:Prims.unit =
-    Rust_primitives.Hax.never_to_any (Core.Panicking.panic "not implemented"
-        <:
-        Rust_primitives.Hax.t_Never)
-  in
-  output
+assume
+val mm256_storeu_si256_u8':
+    output: t_Slice u8 ->
+    vector: Minicore.Abstractions.Bitvec.t_BitVec (mk_u64 256)
+  -> t_Slice u8
 
-let mm256_storeu_si256_i16
-      (output: t_Slice i16)
-      (vector: Minicore.Abstractions.Bitvec.t_BitVec (mk_u64 256))
-    : Prims.Pure (t_Slice i16)
+let mm256_storeu_si256_u8 = mm256_storeu_si256_u8'
+
+assume
+val mm256_storeu_si256_i16':
+    output: t_Slice i16 ->
+    vector: Minicore.Abstractions.Bitvec.t_BitVec (mk_u64 256)
+  -> Prims.Pure (t_Slice i16)
       Prims.l_True
       (ensures
         fun output_future ->
           let output_future:t_Slice i16 = output_future in
           (Core.Slice.impl__len #i16 output_future <: usize) =.
-          (Core.Slice.impl__len #i16 output <: usize)) =
-  let _:Prims.unit =
-    if true
-    then
-      let _:Prims.unit =
-        match Core.Slice.impl__len #i16 output, mk_usize 16 <: (usize & usize) with
-        | left_val, right_val -> Hax_lib.v_assert (left_val =. right_val <: bool)
-      in
-      ()
-  in
-  let _:Prims.unit =
-    Rust_primitives.Hax.never_to_any (Core.Panicking.panic "not implemented"
-        <:
-        Rust_primitives.Hax.t_Never)
-  in
-  output
+          (Core.Slice.impl__len #i16 output <: usize))
 
-let mm256_storeu_si256_i32
-      (output: t_Slice i32)
-      (vector: Minicore.Abstractions.Bitvec.t_BitVec (mk_u64 256))
-    : t_Slice i32 =
-  let _:Prims.unit =
-    if true
-    then
-      let _:Prims.unit =
-        match Core.Slice.impl__len #i32 output, mk_usize 8 <: (usize & usize) with
-        | left_val, right_val -> Hax_lib.v_assert (left_val =. right_val <: bool)
-      in
-      ()
-  in
-  let _:Prims.unit =
-    Rust_primitives.Hax.never_to_any (Core.Panicking.panic "not implemented"
-        <:
-        Rust_primitives.Hax.t_Never)
-  in
-  output
+let mm256_storeu_si256_i16 = mm256_storeu_si256_i16'
 
-let mm_storeu_si128
-      (output: t_Slice i16)
-      (vector: Minicore.Abstractions.Bitvec.t_BitVec (mk_u64 128))
-    : t_Slice i16 =
-  let _:Prims.unit =
-    if true
-    then
-      let _:Prims.unit =
-        Hax_lib.v_assert ((Core.Slice.impl__len #i16 output <: usize) >=. mk_usize 8 <: bool)
-      in
-      ()
-  in
-  let _:Prims.unit =
-    Rust_primitives.Hax.never_to_any (Core.Panicking.panic "not implemented"
-        <:
-        Rust_primitives.Hax.t_Never)
-  in
-  output
+assume
+val mm256_storeu_si256_i32':
+    output: t_Slice i32 ->
+    vector: Minicore.Abstractions.Bitvec.t_BitVec (mk_u64 256)
+  -> t_Slice i32
 
-let mm_storeu_si128_i32
-      (output: t_Slice i32)
-      (vector: Minicore.Abstractions.Bitvec.t_BitVec (mk_u64 128))
-    : t_Slice i32 =
-  let _:Prims.unit =
-    if true
-    then
-      let _:Prims.unit =
-        match Core.Slice.impl__len #i32 output, mk_usize 4 <: (usize & usize) with
-        | left_val, right_val -> Hax_lib.v_assert (left_val =. right_val <: bool)
-      in
-      ()
-  in
-  let _:Prims.unit =
-    Rust_primitives.Hax.never_to_any (Core.Panicking.panic "not implemented"
-        <:
-        Rust_primitives.Hax.t_Never)
-  in
-  output
+let mm256_storeu_si256_i32 = mm256_storeu_si256_i32'
 
-let mm_storeu_bytes_si128
-      (output: t_Slice u8)
-      (vector: Minicore.Abstractions.Bitvec.t_BitVec (mk_u64 128))
-    : t_Slice u8 =
-  let _:Prims.unit =
-    if true
-    then
-      let _:Prims.unit =
-        match Core.Slice.impl__len #u8 output, mk_usize 16 <: (usize & usize) with
-        | left_val, right_val -> Hax_lib.v_assert (left_val =. right_val <: bool)
-      in
-      ()
-  in
-  let _:Prims.unit =
-    Rust_primitives.Hax.never_to_any (Core.Panicking.panic "not implemented"
-        <:
-        Rust_primitives.Hax.t_Never)
-  in
-  output
+assume
+val mm_storeu_si128':
+    output: t_Slice i16 ->
+    vector: Minicore.Abstractions.Bitvec.t_BitVec (mk_u64 128)
+  -> t_Slice i16
 
-let mm_loadu_si128 (input: t_Slice u8) : Minicore.Abstractions.Bitvec.t_BitVec (mk_u64 128) =
-  let _:Prims.unit =
-    if true
-    then
-      let _:Prims.unit =
-        match Core.Slice.impl__len #u8 input, mk_usize 16 <: (usize & usize) with
-        | left_val, right_val -> Hax_lib.v_assert (left_val =. right_val <: bool)
-      in
-      ()
-  in
-  Rust_primitives.Hax.never_to_any (Core.Panicking.panic "not implemented"
-      <:
-      Rust_primitives.Hax.t_Never)
+let mm_storeu_si128 = mm_storeu_si128'
 
-let mm256_loadu_si256_u8 (input: t_Slice u8) : Minicore.Abstractions.Bitvec.t_BitVec (mk_u64 256) =
-  let _:Prims.unit =
-    if true
-    then
-      let _:Prims.unit =
-        match Core.Slice.impl__len #u8 input, mk_usize 32 <: (usize & usize) with
-        | left_val, right_val -> Hax_lib.v_assert (left_val =. right_val <: bool)
-      in
-      ()
-  in
-  Rust_primitives.Hax.never_to_any (Core.Panicking.panic "not implemented"
-      <:
-      Rust_primitives.Hax.t_Never)
+assume
+val mm_storeu_si128_i32':
+    output: t_Slice i32 ->
+    vector: Minicore.Abstractions.Bitvec.t_BitVec (mk_u64 128)
+  -> t_Slice i32
 
-let mm256_loadu_si256_i16 (input: t_Slice i16) : Minicore.Abstractions.Bitvec.t_BitVec (mk_u64 256) =
-  let _:Prims.unit =
-    if true
-    then
-      let _:Prims.unit =
-        match Core.Slice.impl__len #i16 input, mk_usize 16 <: (usize & usize) with
-        | left_val, right_val -> Hax_lib.v_assert (left_val =. right_val <: bool)
-      in
-      ()
-  in
-  Rust_primitives.Hax.never_to_any (Core.Panicking.panic "not implemented"
-      <:
-      Rust_primitives.Hax.t_Never)
+let mm_storeu_si128_i32 = mm_storeu_si128_i32'
 
-let mm256_loadu_si256_i32 (input: t_Slice i32) : Minicore.Abstractions.Bitvec.t_BitVec (mk_u64 256) =
-  let _:Prims.unit =
-    if true
-    then
-      let _:Prims.unit =
-        match Core.Slice.impl__len #i32 input, mk_usize 8 <: (usize & usize) with
-        | left_val, right_val -> Hax_lib.v_assert (left_val =. right_val <: bool)
-      in
-      ()
-  in
-  Rust_primitives.Hax.never_to_any (Core.Panicking.panic "not implemented"
-      <:
-      Rust_primitives.Hax.t_Never)
+assume
+val mm_storeu_bytes_si128':
+    output: t_Slice u8 ->
+    vector: Minicore.Abstractions.Bitvec.t_BitVec (mk_u64 128)
+  -> Prims.Pure (t_Slice u8)
+      Prims.l_True
+      (ensures
+        fun output_future ->
+          let output_future:t_Slice u8 = output_future in
+          (Core.Slice.impl__len #u8 output <: usize) =.
+          (Core.Slice.impl__len #u8 output_future <: usize))
 
-let mm256_setzero_si256 (_: Prims.unit) : Minicore.Abstractions.Bitvec.t_BitVec (mk_u64 256) =
-  Rust_primitives.Hax.never_to_any (Core.Panicking.panic "not implemented"
-      <:
-      Rust_primitives.Hax.t_Never)
+let mm_storeu_bytes_si128 = mm_storeu_bytes_si128'
 
-let mm256_set_m128i (hi lo: Minicore.Abstractions.Bitvec.t_BitVec (mk_u64 128))
-    : Minicore.Abstractions.Bitvec.t_BitVec (mk_u64 256) =
-  Rust_primitives.Hax.never_to_any (Core.Panicking.panic "not implemented"
-      <:
-      Rust_primitives.Hax.t_Never)
+assume
+val mm_loadu_si128': input: t_Slice u8 -> Minicore.Abstractions.Bitvec.t_BitVec (mk_u64 128)
+
+let mm_loadu_si128 = mm_loadu_si128'
+
+assume
+val mm256_loadu_si256_u8': input: t_Slice u8 -> Minicore.Abstractions.Bitvec.t_BitVec (mk_u64 256)
+
+let mm256_loadu_si256_u8 = mm256_loadu_si256_u8'
+
+assume
+val mm256_loadu_si256_i16': input: t_Slice i16 -> Minicore.Abstractions.Bitvec.t_BitVec (mk_u64 256)
+
+let mm256_loadu_si256_i16 = mm256_loadu_si256_i16'
+
+assume
+val mm256_loadu_si256_i32': input: t_Slice i32 -> Minicore.Abstractions.Bitvec.t_BitVec (mk_u64 256)
+
+let mm256_loadu_si256_i32 = mm256_loadu_si256_i32'
+
+assume
+val mm256_setzero_si256': Prims.unit -> Minicore.Abstractions.Bitvec.t_BitVec (mk_u64 256)
+
+let mm256_setzero_si256 = mm256_setzero_si256'
+
+assume
+val mm256_set_m128i':
+    hi: Minicore.Abstractions.Bitvec.t_BitVec (mk_u64 128) ->
+    lo: Minicore.Abstractions.Bitvec.t_BitVec (mk_u64 128)
+  -> Minicore.Abstractions.Bitvec.t_BitVec (mk_u64 256)
+
+let mm256_set_m128i = mm256_set_m128i'
 
 let mm_set_epi8
       (byte15 byte14 byte13 byte12 byte11 byte10 byte9 byte8 byte7 byte6 byte5 byte4 byte3 byte2 byte1 byte0:
           u8)
     : Minicore.Abstractions.Bitvec.t_BitVec (mk_u64 128) =
-  Rust_primitives.Hax.never_to_any (Core.Panicking.panic "not implemented"
-      <:
-      Rust_primitives.Hax.t_Never)
+  Minicore.Arch.X86.e_mm_set_epi8 (cast (byte15 <: u8) <: i8) (cast (byte14 <: u8) <: i8)
+    (cast (byte13 <: u8) <: i8) (cast (byte12 <: u8) <: i8) (cast (byte11 <: u8) <: i8)
+    (cast (byte10 <: u8) <: i8) (cast (byte9 <: u8) <: i8) (cast (byte8 <: u8) <: i8)
+    (cast (byte7 <: u8) <: i8) (cast (byte6 <: u8) <: i8) (cast (byte5 <: u8) <: i8)
+    (cast (byte4 <: u8) <: i8) (cast (byte3 <: u8) <: i8) (cast (byte2 <: u8) <: i8)
+    (cast (byte1 <: u8) <: i8) (cast (byte0 <: u8) <: i8)
 
-let mm256_set_epi8
-      (byte31 byte30 byte29 byte28 byte27 byte26 byte25 byte24 byte23 byte22 byte21 byte20 byte19 byte18 byte17 byte16 byte15 byte14 byte13 byte12 byte11 byte10 byte9 byte8 byte7 byte6 byte5 byte4 byte3 byte2 byte1 byte0:
-          i8)
+assume
+val mm256_set_epi8':
+    byte31: i8 ->
+    byte30: i8 ->
+    byte29: i8 ->
+    byte28: i8 ->
+    byte27: i8 ->
+    byte26: i8 ->
+    byte25: i8 ->
+    byte24: i8 ->
+    byte23: i8 ->
+    byte22: i8 ->
+    byte21: i8 ->
+    byte20: i8 ->
+    byte19: i8 ->
+    byte18: i8 ->
+    byte17: i8 ->
+    byte16: i8 ->
+    byte15: i8 ->
+    byte14: i8 ->
+    byte13: i8 ->
+    byte12: i8 ->
+    byte11: i8 ->
+    byte10: i8 ->
+    byte9: i8 ->
+    byte8: i8 ->
+    byte7: i8 ->
+    byte6: i8 ->
+    byte5: i8 ->
+    byte4: i8 ->
+    byte3: i8 ->
+    byte2: i8 ->
+    byte1: i8 ->
+    byte0: i8
+  -> Minicore.Abstractions.Bitvec.t_BitVec (mk_u64 256)
+
+let mm256_set_epi8 = mm256_set_epi8'
+
+assume
+val mm256_set1_epi16': constant: i16 -> Minicore.Abstractions.Bitvec.t_BitVec (mk_u64 256)
+
+let mm256_set1_epi16 = mm256_set1_epi16'
+
+assume
+val mm256_set_epi16':
+    input15: i16 ->
+    input14: i16 ->
+    input13: i16 ->
+    input12: i16 ->
+    input11: i16 ->
+    input10: i16 ->
+    input9: i16 ->
+    input8: i16 ->
+    input7: i16 ->
+    input6: i16 ->
+    input5: i16 ->
+    input4: i16 ->
+    input3: i16 ->
+    input2: i16 ->
+    input1: i16 ->
+    input0: i16
+  -> Minicore.Abstractions.Bitvec.t_BitVec (mk_u64 256)
+
+let mm256_set_epi16 = mm256_set_epi16'
+
+assume
+val mm_set1_epi16': constant: i16 -> Minicore.Abstractions.Bitvec.t_BitVec (mk_u64 128)
+
+let mm_set1_epi16 = mm_set1_epi16'
+
+assume
+val mm256_set1_epi32': constant: i32 -> Minicore.Abstractions.Bitvec.t_BitVec (mk_u64 256)
+
+let mm256_set1_epi32 = mm256_set1_epi32'
+
+assume
+val mm_set_epi32': input3: i32 -> input2: i32 -> input1: i32 -> input0: i32
+  -> Minicore.Abstractions.Bitvec.t_BitVec (mk_u64 128)
+
+let mm_set_epi32 = mm_set_epi32'
+
+let mm256_set_epi32 (x7 x6 x5 x4 x3 x2 x1 x0: i32)
     : Minicore.Abstractions.Bitvec.t_BitVec (mk_u64 256) =
-  Rust_primitives.Hax.never_to_any (Core.Panicking.panic "not implemented"
-      <:
-      Rust_primitives.Hax.t_Never)
+  Minicore.Arch.X86.e_mm256_set_epi32 x7 x6 x5 x4 x3 x2 x1 x0
 
-let mm256_set1_epi16 (constant: i16) : Minicore.Abstractions.Bitvec.t_BitVec (mk_u64 256) =
-  Rust_primitives.Hax.never_to_any (Core.Panicking.panic "not implemented"
-      <:
-      Rust_primitives.Hax.t_Never)
+assume
+val mm_add_epi16':
+    lhs: Minicore.Abstractions.Bitvec.t_BitVec (mk_u64 128) ->
+    rhs: Minicore.Abstractions.Bitvec.t_BitVec (mk_u64 128)
+  -> Minicore.Abstractions.Bitvec.t_BitVec (mk_u64 128)
 
-let mm256_set_epi16
-      (input15 input14 input13 input12 input11 input10 input9 input8 input7 input6 input5 input4 input3 input2 input1 input0:
-          i16)
-    : Minicore.Abstractions.Bitvec.t_BitVec (mk_u64 256) =
-  Rust_primitives.Hax.never_to_any (Core.Panicking.panic "not implemented"
-      <:
-      Rust_primitives.Hax.t_Never)
+let mm_add_epi16 = mm_add_epi16'
 
-let mm_set1_epi16 (constant: i16) : Minicore.Abstractions.Bitvec.t_BitVec (mk_u64 128) =
-  Rust_primitives.Hax.never_to_any (Core.Panicking.panic "not implemented"
-      <:
-      Rust_primitives.Hax.t_Never)
+assume
+val mm_sub_epi16':
+    lhs: Minicore.Abstractions.Bitvec.t_BitVec (mk_u64 128) ->
+    rhs: Minicore.Abstractions.Bitvec.t_BitVec (mk_u64 128)
+  -> Minicore.Abstractions.Bitvec.t_BitVec (mk_u64 128)
 
-let mm256_set1_epi32 (constant: i32) : Minicore.Abstractions.Bitvec.t_BitVec (mk_u64 256) =
-  Rust_primitives.Hax.never_to_any (Core.Panicking.panic "not implemented"
-      <:
-      Rust_primitives.Hax.t_Never)
+let mm_sub_epi16 = mm_sub_epi16'
 
-let mm_set_epi32 (input3 input2 input1 input0: i32)
-    : Minicore.Abstractions.Bitvec.t_BitVec (mk_u64 128) =
-  Rust_primitives.Hax.never_to_any (Core.Panicking.panic "not implemented"
-      <:
-      Rust_primitives.Hax.t_Never)
+assume
+val mm256_add_epi16':
+    lhs: Minicore.Abstractions.Bitvec.t_BitVec (mk_u64 256) ->
+    rhs: Minicore.Abstractions.Bitvec.t_BitVec (mk_u64 256)
+  -> Minicore.Abstractions.Bitvec.t_BitVec (mk_u64 256)
 
-let mm256_set_epi32 (input7 input6 input5 input4 input3 input2 input1 input0: i32)
-    : Minicore.Abstractions.Bitvec.t_BitVec (mk_u64 256) =
-  Rust_primitives.Hax.never_to_any (Core.Panicking.panic "not implemented"
-      <:
-      Rust_primitives.Hax.t_Never)
+let mm256_add_epi16 = mm256_add_epi16'
 
-let mm_add_epi16 (lhs rhs: Minicore.Abstractions.Bitvec.t_BitVec (mk_u64 128))
-    : Minicore.Abstractions.Bitvec.t_BitVec (mk_u64 128) =
-  Rust_primitives.Hax.never_to_any (Core.Panicking.panic "not implemented"
-      <:
-      Rust_primitives.Hax.t_Never)
+assume
+val mm256_madd_epi16':
+    lhs: Minicore.Abstractions.Bitvec.t_BitVec (mk_u64 256) ->
+    rhs: Minicore.Abstractions.Bitvec.t_BitVec (mk_u64 256)
+  -> Minicore.Abstractions.Bitvec.t_BitVec (mk_u64 256)
 
-let mm_sub_epi16 (lhs rhs: Minicore.Abstractions.Bitvec.t_BitVec (mk_u64 128))
-    : Minicore.Abstractions.Bitvec.t_BitVec (mk_u64 128) =
-  Rust_primitives.Hax.never_to_any (Core.Panicking.panic "not implemented"
-      <:
-      Rust_primitives.Hax.t_Never)
+let mm256_madd_epi16 = mm256_madd_epi16'
 
-let mm256_add_epi16 (lhs rhs: Minicore.Abstractions.Bitvec.t_BitVec (mk_u64 256))
-    : Minicore.Abstractions.Bitvec.t_BitVec (mk_u64 256) =
-  Rust_primitives.Hax.never_to_any (Core.Panicking.panic "not implemented"
-      <:
-      Rust_primitives.Hax.t_Never)
+assume
+val mm256_add_epi32':
+    lhs: Minicore.Abstractions.Bitvec.t_BitVec (mk_u64 256) ->
+    rhs: Minicore.Abstractions.Bitvec.t_BitVec (mk_u64 256)
+  -> Minicore.Abstractions.Bitvec.t_BitVec (mk_u64 256)
 
-let mm256_madd_epi16 (lhs rhs: Minicore.Abstractions.Bitvec.t_BitVec (mk_u64 256))
-    : Minicore.Abstractions.Bitvec.t_BitVec (mk_u64 256) =
-  Rust_primitives.Hax.never_to_any (Core.Panicking.panic "not implemented"
-      <:
-      Rust_primitives.Hax.t_Never)
-
-let mm256_add_epi32 (lhs rhs: Minicore.Abstractions.Bitvec.t_BitVec (mk_u64 256))
-    : Minicore.Abstractions.Bitvec.t_BitVec (mk_u64 256) =
-  Rust_primitives.Hax.never_to_any (Core.Panicking.panic "not implemented"
-      <:
-      Rust_primitives.Hax.t_Never)
+let mm256_add_epi32 = mm256_add_epi32'
 
 let mm256_sub_epi16 (lhs rhs: Minicore.Abstractions.Bitvec.t_BitVec (mk_u64 256))
     : Minicore.Abstractions.Bitvec.t_BitVec (mk_u64 256) =
@@ -282,194 +238,189 @@ let mm256_sub_epi16 (lhs rhs: Minicore.Abstractions.Bitvec.t_BitVec (mk_u64 256)
       <:
       Rust_primitives.Hax.t_Never)
 
-let mm256_add_epi64 (lhs rhs: Minicore.Abstractions.Bitvec.t_BitVec (mk_u64 256))
-    : Minicore.Abstractions.Bitvec.t_BitVec (mk_u64 256) =
-  Rust_primitives.Hax.never_to_any (Core.Panicking.panic "not implemented"
-      <:
-      Rust_primitives.Hax.t_Never)
+assume
+val mm256_add_epi64':
+    lhs: Minicore.Abstractions.Bitvec.t_BitVec (mk_u64 256) ->
+    rhs: Minicore.Abstractions.Bitvec.t_BitVec (mk_u64 256)
+  -> Minicore.Abstractions.Bitvec.t_BitVec (mk_u64 256)
 
-let mm256_abs_epi32 (a: Minicore.Abstractions.Bitvec.t_BitVec (mk_u64 256))
-    : Minicore.Abstractions.Bitvec.t_BitVec (mk_u64 256) =
-  Rust_primitives.Hax.never_to_any (Core.Panicking.panic "not implemented"
-      <:
-      Rust_primitives.Hax.t_Never)
+let mm256_add_epi64 = mm256_add_epi64'
 
-let mm256_sub_epi32 (lhs rhs: Minicore.Abstractions.Bitvec.t_BitVec (mk_u64 256))
-    : Minicore.Abstractions.Bitvec.t_BitVec (mk_u64 256) =
-  Rust_primitives.Hax.never_to_any (Core.Panicking.panic "not implemented"
-      <:
-      Rust_primitives.Hax.t_Never)
+assume
+val mm256_abs_epi32': a: Minicore.Abstractions.Bitvec.t_BitVec (mk_u64 256)
+  -> Minicore.Abstractions.Bitvec.t_BitVec (mk_u64 256)
 
-let mm256_mullo_epi16 (lhs rhs: Minicore.Abstractions.Bitvec.t_BitVec (mk_u64 256))
-    : Minicore.Abstractions.Bitvec.t_BitVec (mk_u64 256) =
-  Rust_primitives.Hax.never_to_any (Core.Panicking.panic "not implemented"
-      <:
-      Rust_primitives.Hax.t_Never)
+let mm256_abs_epi32 = mm256_abs_epi32'
 
-let mm_mullo_epi16 (lhs rhs: Minicore.Abstractions.Bitvec.t_BitVec (mk_u64 128))
-    : Minicore.Abstractions.Bitvec.t_BitVec (mk_u64 128) =
-  Rust_primitives.Hax.never_to_any (Core.Panicking.panic "not implemented"
-      <:
-      Rust_primitives.Hax.t_Never)
+assume
+val mm256_sub_epi32':
+    lhs: Minicore.Abstractions.Bitvec.t_BitVec (mk_u64 256) ->
+    rhs: Minicore.Abstractions.Bitvec.t_BitVec (mk_u64 256)
+  -> Minicore.Abstractions.Bitvec.t_BitVec (mk_u64 256)
 
-let mm256_cmpgt_epi16 (lhs rhs: Minicore.Abstractions.Bitvec.t_BitVec (mk_u64 256))
-    : Minicore.Abstractions.Bitvec.t_BitVec (mk_u64 256) =
-  Rust_primitives.Hax.never_to_any (Core.Panicking.panic "not implemented"
-      <:
-      Rust_primitives.Hax.t_Never)
+let mm256_sub_epi32 = mm256_sub_epi32'
 
-let mm256_cmpgt_epi32 (lhs rhs: Minicore.Abstractions.Bitvec.t_BitVec (mk_u64 256))
-    : Minicore.Abstractions.Bitvec.t_BitVec (mk_u64 256) =
-  Rust_primitives.Hax.never_to_any (Core.Panicking.panic "not implemented"
-      <:
-      Rust_primitives.Hax.t_Never)
+assume
+val mm256_mullo_epi16':
+    lhs: Minicore.Abstractions.Bitvec.t_BitVec (mk_u64 256) ->
+    rhs: Minicore.Abstractions.Bitvec.t_BitVec (mk_u64 256)
+  -> Minicore.Abstractions.Bitvec.t_BitVec (mk_u64 256)
 
-let mm256_cmpeq_epi32 (a b: Minicore.Abstractions.Bitvec.t_BitVec (mk_u64 256))
-    : Minicore.Abstractions.Bitvec.t_BitVec (mk_u64 256) =
-  Rust_primitives.Hax.never_to_any (Core.Panicking.panic "not implemented"
-      <:
-      Rust_primitives.Hax.t_Never)
+let mm256_mullo_epi16 = mm256_mullo_epi16'
 
-let mm256_sign_epi32 (a b: Minicore.Abstractions.Bitvec.t_BitVec (mk_u64 256))
-    : Minicore.Abstractions.Bitvec.t_BitVec (mk_u64 256) =
-  Rust_primitives.Hax.never_to_any (Core.Panicking.panic "not implemented"
-      <:
-      Rust_primitives.Hax.t_Never)
+assume
+val mm_mullo_epi16':
+    lhs: Minicore.Abstractions.Bitvec.t_BitVec (mk_u64 128) ->
+    rhs: Minicore.Abstractions.Bitvec.t_BitVec (mk_u64 128)
+  -> Minicore.Abstractions.Bitvec.t_BitVec (mk_u64 128)
 
-let mm256_castsi256_ps (a: Minicore.Abstractions.Bitvec.t_BitVec (mk_u64 256)) : u8 =
-  Rust_primitives.Hax.never_to_any (Core.Panicking.panic "not implemented"
-      <:
-      Rust_primitives.Hax.t_Never)
+let mm_mullo_epi16 = mm_mullo_epi16'
 
-let mm256_movemask_ps (a: u8) : i32 =
-  Rust_primitives.Hax.never_to_any (Core.Panicking.panic "not implemented"
-      <:
-      Rust_primitives.Hax.t_Never)
+assume
+val mm256_cmpgt_epi16':
+    lhs: Minicore.Abstractions.Bitvec.t_BitVec (mk_u64 256) ->
+    rhs: Minicore.Abstractions.Bitvec.t_BitVec (mk_u64 256)
+  -> Minicore.Abstractions.Bitvec.t_BitVec (mk_u64 256)
 
-let mm_mulhi_epi16 (lhs rhs: Minicore.Abstractions.Bitvec.t_BitVec (mk_u64 128))
-    : Minicore.Abstractions.Bitvec.t_BitVec (mk_u64 128) =
-  Rust_primitives.Hax.never_to_any (Core.Panicking.panic "not implemented"
-      <:
-      Rust_primitives.Hax.t_Never)
+let mm256_cmpgt_epi16 = mm256_cmpgt_epi16'
 
-let mm256_mullo_epi32 (lhs rhs: Minicore.Abstractions.Bitvec.t_BitVec (mk_u64 256))
-    : Minicore.Abstractions.Bitvec.t_BitVec (mk_u64 256) =
-  Rust_primitives.Hax.never_to_any (Core.Panicking.panic "not implemented"
-      <:
-      Rust_primitives.Hax.t_Never)
+assume
+val mm256_cmpgt_epi32':
+    lhs: Minicore.Abstractions.Bitvec.t_BitVec (mk_u64 256) ->
+    rhs: Minicore.Abstractions.Bitvec.t_BitVec (mk_u64 256)
+  -> Minicore.Abstractions.Bitvec.t_BitVec (mk_u64 256)
 
-let mm256_mulhi_epi16 (lhs rhs: Minicore.Abstractions.Bitvec.t_BitVec (mk_u64 256))
-    : Minicore.Abstractions.Bitvec.t_BitVec (mk_u64 256) =
-  Rust_primitives.Hax.never_to_any (Core.Panicking.panic "not implemented"
-      <:
-      Rust_primitives.Hax.t_Never)
+let mm256_cmpgt_epi32 = mm256_cmpgt_epi32'
 
-let mm256_mul_epu32 (lhs rhs: Minicore.Abstractions.Bitvec.t_BitVec (mk_u64 256))
-    : Minicore.Abstractions.Bitvec.t_BitVec (mk_u64 256) =
-  Rust_primitives.Hax.never_to_any (Core.Panicking.panic "not implemented"
-      <:
-      Rust_primitives.Hax.t_Never)
+assume
+val mm256_cmpeq_epi32':
+    a: Minicore.Abstractions.Bitvec.t_BitVec (mk_u64 256) ->
+    b: Minicore.Abstractions.Bitvec.t_BitVec (mk_u64 256)
+  -> Minicore.Abstractions.Bitvec.t_BitVec (mk_u64 256)
 
-let mm256_mul_epi32 (lhs rhs: Minicore.Abstractions.Bitvec.t_BitVec (mk_u64 256))
-    : Minicore.Abstractions.Bitvec.t_BitVec (mk_u64 256) =
-  Rust_primitives.Hax.never_to_any (Core.Panicking.panic "not implemented"
-      <:
-      Rust_primitives.Hax.t_Never)
+let mm256_cmpeq_epi32 = mm256_cmpeq_epi32'
 
-let mm256_and_si256 (lhs rhs: Minicore.Abstractions.Bitvec.t_BitVec (mk_u64 256))
-    : Minicore.Abstractions.Bitvec.t_BitVec (mk_u64 256) =
-  Rust_primitives.Hax.never_to_any (Core.Panicking.panic "not implemented"
-      <:
-      Rust_primitives.Hax.t_Never)
+assume
+val mm256_sign_epi32':
+    a: Minicore.Abstractions.Bitvec.t_BitVec (mk_u64 256) ->
+    b: Minicore.Abstractions.Bitvec.t_BitVec (mk_u64 256)
+  -> Minicore.Abstractions.Bitvec.t_BitVec (mk_u64 256)
 
-let mm256_or_si256 (a b: Minicore.Abstractions.Bitvec.t_BitVec (mk_u64 256))
-    : Minicore.Abstractions.Bitvec.t_BitVec (mk_u64 256) =
-  Rust_primitives.Hax.never_to_any (Core.Panicking.panic "not implemented"
-      <:
-      Rust_primitives.Hax.t_Never)
+let mm256_sign_epi32 = mm256_sign_epi32'
 
-let mm256_testz_si256 (lhs rhs: Minicore.Abstractions.Bitvec.t_BitVec (mk_u64 256)) : i32 =
-  Rust_primitives.Hax.never_to_any (Core.Panicking.panic "not implemented"
-      <:
-      Rust_primitives.Hax.t_Never)
+assume
+val mm256_castsi256_ps': a: Minicore.Abstractions.Bitvec.t_BitVec (mk_u64 256) -> u8
 
-let mm256_xor_si256 (lhs rhs: Minicore.Abstractions.Bitvec.t_BitVec (mk_u64 256))
-    : Minicore.Abstractions.Bitvec.t_BitVec (mk_u64 256) =
-  Rust_primitives.Hax.never_to_any (Core.Panicking.panic "not implemented"
-      <:
-      Rust_primitives.Hax.t_Never)
+let mm256_castsi256_ps = mm256_castsi256_ps'
 
-let mm256_srai_epi16 (v_SHIFT_BY: i32) (vector: Minicore.Abstractions.Bitvec.t_BitVec (mk_u64 256))
-    : Prims.Pure (Minicore.Abstractions.Bitvec.t_BitVec (mk_u64 256))
+assume
+val mm256_movemask_ps': a: u8 -> i32
+
+let mm256_movemask_ps = mm256_movemask_ps'
+
+assume
+val mm_mulhi_epi16':
+    lhs: Minicore.Abstractions.Bitvec.t_BitVec (mk_u64 128) ->
+    rhs: Minicore.Abstractions.Bitvec.t_BitVec (mk_u64 128)
+  -> Minicore.Abstractions.Bitvec.t_BitVec (mk_u64 128)
+
+let mm_mulhi_epi16 = mm_mulhi_epi16'
+
+assume
+val mm256_mullo_epi32':
+    lhs: Minicore.Abstractions.Bitvec.t_BitVec (mk_u64 256) ->
+    rhs: Minicore.Abstractions.Bitvec.t_BitVec (mk_u64 256)
+  -> Minicore.Abstractions.Bitvec.t_BitVec (mk_u64 256)
+
+let mm256_mullo_epi32 = mm256_mullo_epi32'
+
+assume
+val mm256_mulhi_epi16':
+    lhs: Minicore.Abstractions.Bitvec.t_BitVec (mk_u64 256) ->
+    rhs: Minicore.Abstractions.Bitvec.t_BitVec (mk_u64 256)
+  -> Minicore.Abstractions.Bitvec.t_BitVec (mk_u64 256)
+
+let mm256_mulhi_epi16 = mm256_mulhi_epi16'
+
+assume
+val mm256_mul_epu32':
+    lhs: Minicore.Abstractions.Bitvec.t_BitVec (mk_u64 256) ->
+    rhs: Minicore.Abstractions.Bitvec.t_BitVec (mk_u64 256)
+  -> Minicore.Abstractions.Bitvec.t_BitVec (mk_u64 256)
+
+let mm256_mul_epu32 = mm256_mul_epu32'
+
+assume
+val mm256_mul_epi32':
+    lhs: Minicore.Abstractions.Bitvec.t_BitVec (mk_u64 256) ->
+    rhs: Minicore.Abstractions.Bitvec.t_BitVec (mk_u64 256)
+  -> Minicore.Abstractions.Bitvec.t_BitVec (mk_u64 256)
+
+let mm256_mul_epi32 = mm256_mul_epi32'
+
+assume
+val mm256_and_si256':
+    lhs: Minicore.Abstractions.Bitvec.t_BitVec (mk_u64 256) ->
+    rhs: Minicore.Abstractions.Bitvec.t_BitVec (mk_u64 256)
+  -> Minicore.Abstractions.Bitvec.t_BitVec (mk_u64 256)
+
+let mm256_and_si256 = mm256_and_si256'
+
+assume
+val mm256_or_si256':
+    a: Minicore.Abstractions.Bitvec.t_BitVec (mk_u64 256) ->
+    b: Minicore.Abstractions.Bitvec.t_BitVec (mk_u64 256)
+  -> Minicore.Abstractions.Bitvec.t_BitVec (mk_u64 256)
+
+let mm256_or_si256 = mm256_or_si256'
+
+assume
+val mm256_testz_si256':
+    lhs: Minicore.Abstractions.Bitvec.t_BitVec (mk_u64 256) ->
+    rhs: Minicore.Abstractions.Bitvec.t_BitVec (mk_u64 256)
+  -> i32
+
+let mm256_testz_si256 = mm256_testz_si256'
+
+assume
+val mm256_xor_si256':
+    lhs: Minicore.Abstractions.Bitvec.t_BitVec (mk_u64 256) ->
+    rhs: Minicore.Abstractions.Bitvec.t_BitVec (mk_u64 256)
+  -> Minicore.Abstractions.Bitvec.t_BitVec (mk_u64 256)
+
+let mm256_xor_si256 = mm256_xor_si256'
+
+assume
+val mm256_srai_epi16': v_SHIFT_BY: i32 -> vector: Minicore.Abstractions.Bitvec.t_BitVec (mk_u64 256)
+  -> Prims.Pure (Minicore.Abstractions.Bitvec.t_BitVec (mk_u64 256))
       (requires v_SHIFT_BY >=. mk_i32 0 && v_SHIFT_BY <. mk_i32 16)
-      (fun _ -> Prims.l_True) =
-  let _:Prims.unit =
-    if true
-    then
-      let _:Prims.unit =
-        Hax_lib.v_assert ((v_SHIFT_BY >=. mk_i32 0 <: bool) && (v_SHIFT_BY <. mk_i32 16 <: bool))
-      in
-      ()
-  in
-  Rust_primitives.Hax.never_to_any (Core.Panicking.panic "not implemented"
-      <:
-      Rust_primitives.Hax.t_Never)
+      (fun _ -> Prims.l_True)
 
-let mm256_srai_epi32 (v_SHIFT_BY: i32) (vector: Minicore.Abstractions.Bitvec.t_BitVec (mk_u64 256))
-    : Minicore.Abstractions.Bitvec.t_BitVec (mk_u64 256) =
-  let _:Prims.unit =
-    if true
-    then
-      let _:Prims.unit =
-        Hax_lib.v_assert ((v_SHIFT_BY >=. mk_i32 0 <: bool) && (v_SHIFT_BY <. mk_i32 32 <: bool))
-      in
-      ()
-  in
-  Rust_primitives.Hax.never_to_any (Core.Panicking.panic "not implemented"
-      <:
-      Rust_primitives.Hax.t_Never)
+let mm256_srai_epi16 (v_SHIFT_BY: i32) = mm256_srai_epi16' v_SHIFT_BY
 
-let mm256_srli_epi16 (v_SHIFT_BY: i32) (vector: Minicore.Abstractions.Bitvec.t_BitVec (mk_u64 256))
-    : Minicore.Abstractions.Bitvec.t_BitVec (mk_u64 256) =
-  let _:Prims.unit =
-    if true
-    then
-      let _:Prims.unit =
-        Hax_lib.v_assert ((v_SHIFT_BY >=. mk_i32 0 <: bool) && (v_SHIFT_BY <. mk_i32 16 <: bool))
-      in
-      ()
-  in
-  Rust_primitives.Hax.never_to_any (Core.Panicking.panic "not implemented"
-      <:
-      Rust_primitives.Hax.t_Never)
+assume
+val mm256_srai_epi32': v_SHIFT_BY: i32 -> vector: Minicore.Abstractions.Bitvec.t_BitVec (mk_u64 256)
+  -> Minicore.Abstractions.Bitvec.t_BitVec (mk_u64 256)
 
-let mm256_srli_epi32 (v_SHIFT_BY: i32) (vector: Minicore.Abstractions.Bitvec.t_BitVec (mk_u64 256))
-    : Minicore.Abstractions.Bitvec.t_BitVec (mk_u64 256) =
-  let _:Prims.unit =
-    if true
-    then
-      let _:Prims.unit =
-        Hax_lib.v_assert ((v_SHIFT_BY >=. mk_i32 0 <: bool) && (v_SHIFT_BY <. mk_i32 32 <: bool))
-      in
-      ()
-  in
-  Rust_primitives.Hax.never_to_any (Core.Panicking.panic "not implemented"
-      <:
-      Rust_primitives.Hax.t_Never)
+let mm256_srai_epi32 (v_SHIFT_BY: i32) = mm256_srai_epi32' v_SHIFT_BY
 
-let mm_srli_epi64 (v_SHIFT_BY: i32) (vector: Minicore.Abstractions.Bitvec.t_BitVec (mk_u64 128))
-    : Minicore.Abstractions.Bitvec.t_BitVec (mk_u64 128) =
-  let _:Prims.unit =
-    if true
-    then
-      let _:Prims.unit =
-        Hax_lib.v_assert ((v_SHIFT_BY >=. mk_i32 0 <: bool) && (v_SHIFT_BY <. mk_i32 64 <: bool))
-      in
-      ()
-  in
-  Rust_primitives.Hax.never_to_any (Core.Panicking.panic "not implemented"
-      <:
-      Rust_primitives.Hax.t_Never)
+assume
+val mm256_srli_epi16': v_SHIFT_BY: i32 -> vector: Minicore.Abstractions.Bitvec.t_BitVec (mk_u64 256)
+  -> Minicore.Abstractions.Bitvec.t_BitVec (mk_u64 256)
+
+let mm256_srli_epi16 (v_SHIFT_BY: i32) = mm256_srli_epi16' v_SHIFT_BY
+
+assume
+val mm256_srli_epi32': v_SHIFT_BY: i32 -> vector: Minicore.Abstractions.Bitvec.t_BitVec (mk_u64 256)
+  -> Minicore.Abstractions.Bitvec.t_BitVec (mk_u64 256)
+
+let mm256_srli_epi32 (v_SHIFT_BY: i32) = mm256_srli_epi32' v_SHIFT_BY
+
+assume
+val mm_srli_epi64': v_SHIFT_BY: i32 -> vector: Minicore.Abstractions.Bitvec.t_BitVec (mk_u64 128)
+  -> Minicore.Abstractions.Bitvec.t_BitVec (mk_u64 128)
+
+let mm_srli_epi64 (v_SHIFT_BY: i32) = mm_srli_epi64' v_SHIFT_BY
 
 let mm256_srli_epi64 (v_SHIFT_BY: i32) (vector: Minicore.Abstractions.Bitvec.t_BitVec (mk_u64 256))
     : Minicore.Abstractions.Bitvec.t_BitVec (mk_u64 256) =
@@ -479,257 +430,221 @@ let mm256_slli_epi16 (v_SHIFT_BY: i32) (vector: Minicore.Abstractions.Bitvec.t_B
     : Minicore.Abstractions.Bitvec.t_BitVec (mk_u64 256) =
   Minicore.Arch.X86.e_mm256_slli_epi16 v_SHIFT_BY vector
 
-let mm256_slli_epi32 (v_SHIFT_BY: i32) (vector: Minicore.Abstractions.Bitvec.t_BitVec (mk_u64 256))
-    : Minicore.Abstractions.Bitvec.t_BitVec (mk_u64 256) =
-  let _:Prims.unit =
-    if true
-    then
-      let _:Prims.unit =
-        Hax_lib.v_assert ((v_SHIFT_BY >=. mk_i32 0 <: bool) && (v_SHIFT_BY <. mk_i32 32 <: bool))
-      in
-      ()
-  in
-  Rust_primitives.Hax.never_to_any (Core.Panicking.panic "not implemented"
-      <:
-      Rust_primitives.Hax.t_Never)
+assume
+val mm256_slli_epi32': v_SHIFT_BY: i32 -> vector: Minicore.Abstractions.Bitvec.t_BitVec (mk_u64 256)
+  -> Minicore.Abstractions.Bitvec.t_BitVec (mk_u64 256)
+
+let mm256_slli_epi32 (v_SHIFT_BY: i32) = mm256_slli_epi32' v_SHIFT_BY
 
 let mm_shuffle_epi8 (vector control: Minicore.Abstractions.Bitvec.t_BitVec (mk_u64 128))
     : Minicore.Abstractions.Bitvec.t_BitVec (mk_u64 128) =
-  Rust_primitives.Hax.never_to_any (Core.Panicking.panic "not implemented"
-      <:
-      Rust_primitives.Hax.t_Never)
+  Minicore.Arch.X86.e_mm_shuffle_epi8 vector control
 
-let mm256_shuffle_epi8 (vector control: Minicore.Abstractions.Bitvec.t_BitVec (mk_u64 256))
-    : Minicore.Abstractions.Bitvec.t_BitVec (mk_u64 256) =
-  Rust_primitives.Hax.never_to_any (Core.Panicking.panic "not implemented"
-      <:
-      Rust_primitives.Hax.t_Never)
+assume
+val mm256_shuffle_epi8':
+    vector: Minicore.Abstractions.Bitvec.t_BitVec (mk_u64 256) ->
+    control: Minicore.Abstractions.Bitvec.t_BitVec (mk_u64 256)
+  -> Minicore.Abstractions.Bitvec.t_BitVec (mk_u64 256)
 
-let mm256_shuffle_epi32
-      (v_CONTROL: i32)
-      (vector: Minicore.Abstractions.Bitvec.t_BitVec (mk_u64 256))
-    : Minicore.Abstractions.Bitvec.t_BitVec (mk_u64 256) =
-  let _:Prims.unit =
-    if true
-    then
-      let _:Prims.unit =
-        Hax_lib.v_assert ((v_CONTROL >=. mk_i32 0 <: bool) && (v_CONTROL <. mk_i32 256 <: bool))
-      in
-      ()
-  in
-  Rust_primitives.Hax.never_to_any (Core.Panicking.panic "not implemented"
-      <:
-      Rust_primitives.Hax.t_Never)
+let mm256_shuffle_epi8 = mm256_shuffle_epi8'
 
-let mm256_permute4x64_epi64
-      (v_CONTROL: i32)
-      (vector: Minicore.Abstractions.Bitvec.t_BitVec (mk_u64 256))
-    : Minicore.Abstractions.Bitvec.t_BitVec (mk_u64 256) =
-  let _:Prims.unit =
-    if true
-    then
-      let _:Prims.unit =
-        Hax_lib.v_assert ((v_CONTROL >=. mk_i32 0 <: bool) && (v_CONTROL <. mk_i32 256 <: bool))
-      in
-      ()
-  in
-  Rust_primitives.Hax.never_to_any (Core.Panicking.panic "not implemented"
-      <:
-      Rust_primitives.Hax.t_Never)
+assume
+val mm256_shuffle_epi32':
+    v_CONTROL: i32 ->
+    vector: Minicore.Abstractions.Bitvec.t_BitVec (mk_u64 256)
+  -> Minicore.Abstractions.Bitvec.t_BitVec (mk_u64 256)
 
-let mm256_unpackhi_epi64 (lhs rhs: Minicore.Abstractions.Bitvec.t_BitVec (mk_u64 256))
-    : Minicore.Abstractions.Bitvec.t_BitVec (mk_u64 256) =
-  Rust_primitives.Hax.never_to_any (Core.Panicking.panic "not implemented"
-      <:
-      Rust_primitives.Hax.t_Never)
+let mm256_shuffle_epi32 (v_CONTROL: i32) = mm256_shuffle_epi32' v_CONTROL
 
-let mm256_unpacklo_epi32 (lhs rhs: Minicore.Abstractions.Bitvec.t_BitVec (mk_u64 256))
-    : Minicore.Abstractions.Bitvec.t_BitVec (mk_u64 256) =
-  Rust_primitives.Hax.never_to_any (Core.Panicking.panic "not implemented"
-      <:
-      Rust_primitives.Hax.t_Never)
+assume
+val mm256_permute4x64_epi64':
+    v_CONTROL: i32 ->
+    vector: Minicore.Abstractions.Bitvec.t_BitVec (mk_u64 256)
+  -> Minicore.Abstractions.Bitvec.t_BitVec (mk_u64 256)
 
-let mm256_unpackhi_epi32 (lhs rhs: Minicore.Abstractions.Bitvec.t_BitVec (mk_u64 256))
-    : Minicore.Abstractions.Bitvec.t_BitVec (mk_u64 256) =
-  Rust_primitives.Hax.never_to_any (Core.Panicking.panic "not implemented"
-      <:
-      Rust_primitives.Hax.t_Never)
+let mm256_permute4x64_epi64 (v_CONTROL: i32) = mm256_permute4x64_epi64' v_CONTROL
+
+assume
+val mm256_unpackhi_epi64':
+    lhs: Minicore.Abstractions.Bitvec.t_BitVec (mk_u64 256) ->
+    rhs: Minicore.Abstractions.Bitvec.t_BitVec (mk_u64 256)
+  -> Minicore.Abstractions.Bitvec.t_BitVec (mk_u64 256)
+
+let mm256_unpackhi_epi64 = mm256_unpackhi_epi64'
+
+assume
+val mm256_unpacklo_epi32':
+    lhs: Minicore.Abstractions.Bitvec.t_BitVec (mk_u64 256) ->
+    rhs: Minicore.Abstractions.Bitvec.t_BitVec (mk_u64 256)
+  -> Minicore.Abstractions.Bitvec.t_BitVec (mk_u64 256)
+
+let mm256_unpacklo_epi32 = mm256_unpacklo_epi32'
+
+assume
+val mm256_unpackhi_epi32':
+    lhs: Minicore.Abstractions.Bitvec.t_BitVec (mk_u64 256) ->
+    rhs: Minicore.Abstractions.Bitvec.t_BitVec (mk_u64 256)
+  -> Minicore.Abstractions.Bitvec.t_BitVec (mk_u64 256)
+
+let mm256_unpackhi_epi32 = mm256_unpackhi_epi32'
 
 let mm256_castsi256_si128 (vector: Minicore.Abstractions.Bitvec.t_BitVec (mk_u64 256))
     : Minicore.Abstractions.Bitvec.t_BitVec (mk_u64 128) =
   Minicore.Arch.X86.e_mm256_castsi256_si128 vector
 
-let mm256_castsi128_si256 (vector: Minicore.Abstractions.Bitvec.t_BitVec (mk_u64 128))
-    : Minicore.Abstractions.Bitvec.t_BitVec (mk_u64 256) =
-  Rust_primitives.Hax.never_to_any (Core.Panicking.panic "not implemented"
-      <:
-      Rust_primitives.Hax.t_Never)
+assume
+val mm256_castsi128_si256': vector: Minicore.Abstractions.Bitvec.t_BitVec (mk_u64 128)
+  -> Minicore.Abstractions.Bitvec.t_BitVec (mk_u64 256)
 
-let mm256_cvtepi16_epi32 (vector: Minicore.Abstractions.Bitvec.t_BitVec (mk_u64 128))
-    : Minicore.Abstractions.Bitvec.t_BitVec (mk_u64 256) =
-  Rust_primitives.Hax.never_to_any (Core.Panicking.panic "not implemented"
-      <:
-      Rust_primitives.Hax.t_Never)
+let mm256_castsi128_si256 = mm256_castsi128_si256'
 
-let mm_packs_epi16 (lhs rhs: Minicore.Abstractions.Bitvec.t_BitVec (mk_u64 128))
-    : Minicore.Abstractions.Bitvec.t_BitVec (mk_u64 128) =
-  Rust_primitives.Hax.never_to_any (Core.Panicking.panic "not implemented"
-      <:
-      Rust_primitives.Hax.t_Never)
+assume
+val mm256_cvtepi16_epi32': vector: Minicore.Abstractions.Bitvec.t_BitVec (mk_u64 128)
+  -> Minicore.Abstractions.Bitvec.t_BitVec (mk_u64 256)
 
-let mm256_packs_epi32 (lhs rhs: Minicore.Abstractions.Bitvec.t_BitVec (mk_u64 256))
-    : Minicore.Abstractions.Bitvec.t_BitVec (mk_u64 256) =
-  Rust_primitives.Hax.never_to_any (Core.Panicking.panic "not implemented"
-      <:
-      Rust_primitives.Hax.t_Never)
+let mm256_cvtepi16_epi32 = mm256_cvtepi16_epi32'
 
-let mm256_extracti128_si256
-      (v_CONTROL: i32)
-      (vector: Minicore.Abstractions.Bitvec.t_BitVec (mk_u64 256))
-    : Minicore.Abstractions.Bitvec.t_BitVec (mk_u64 128) =
-  let _:Prims.unit =
-    if true
-    then
-      let _:Prims.unit =
-        Hax_lib.v_assert ((v_CONTROL =. mk_i32 0 <: bool) || (v_CONTROL =. mk_i32 1 <: bool))
-      in
-      ()
-  in
-  Rust_primitives.Hax.never_to_any (Core.Panicking.panic "not implemented"
-      <:
-      Rust_primitives.Hax.t_Never)
+assume
+val mm_packs_epi16':
+    lhs: Minicore.Abstractions.Bitvec.t_BitVec (mk_u64 128) ->
+    rhs: Minicore.Abstractions.Bitvec.t_BitVec (mk_u64 128)
+  -> Minicore.Abstractions.Bitvec.t_BitVec (mk_u64 128)
 
-let mm256_inserti128_si256
-      (v_CONTROL: i32)
-      (vector: Minicore.Abstractions.Bitvec.t_BitVec (mk_u64 256))
-      (vector_i128: Minicore.Abstractions.Bitvec.t_BitVec (mk_u64 128))
-    : Minicore.Abstractions.Bitvec.t_BitVec (mk_u64 256) =
-  let _:Prims.unit =
-    if true
-    then
-      let _:Prims.unit =
-        Hax_lib.v_assert ((v_CONTROL =. mk_i32 0 <: bool) || (v_CONTROL =. mk_i32 1 <: bool))
-      in
-      ()
-  in
-  Rust_primitives.Hax.never_to_any (Core.Panicking.panic "not implemented"
-      <:
-      Rust_primitives.Hax.t_Never)
+let mm_packs_epi16 = mm_packs_epi16'
 
-let mm256_blend_epi16 (v_CONTROL: i32) (lhs rhs: Minicore.Abstractions.Bitvec.t_BitVec (mk_u64 256))
-    : Minicore.Abstractions.Bitvec.t_BitVec (mk_u64 256) =
-  let _:Prims.unit =
-    if true
-    then
-      let _:Prims.unit =
-        Hax_lib.v_assert ((v_CONTROL >=. mk_i32 0 <: bool) && (v_CONTROL <. mk_i32 256 <: bool))
-      in
-      ()
-  in
-  Rust_primitives.Hax.never_to_any (Core.Panicking.panic "not implemented"
-      <:
-      Rust_primitives.Hax.t_Never)
+assume
+val mm256_packs_epi32':
+    lhs: Minicore.Abstractions.Bitvec.t_BitVec (mk_u64 256) ->
+    rhs: Minicore.Abstractions.Bitvec.t_BitVec (mk_u64 256)
+  -> Minicore.Abstractions.Bitvec.t_BitVec (mk_u64 256)
 
-let mm256_blend_epi32 (v_CONTROL: i32) (lhs rhs: Minicore.Abstractions.Bitvec.t_BitVec (mk_u64 256))
-    : Minicore.Abstractions.Bitvec.t_BitVec (mk_u64 256) =
-  let _:Prims.unit =
-    if true
-    then
-      let _:Prims.unit =
-        Hax_lib.v_assert ((v_CONTROL >=. mk_i32 0 <: bool) && (v_CONTROL <. mk_i32 256 <: bool))
-      in
-      ()
-  in
-  Rust_primitives.Hax.never_to_any (Core.Panicking.panic "not implemented"
-      <:
-      Rust_primitives.Hax.t_Never)
+let mm256_packs_epi32 = mm256_packs_epi32'
 
-let vec256_blendv_epi32 (a b mask: Minicore.Abstractions.Bitvec.t_BitVec (mk_u64 256))
-    : Minicore.Abstractions.Bitvec.t_BitVec (mk_u64 256) =
-  Rust_primitives.Hax.never_to_any (Core.Panicking.panic "not implemented"
-      <:
-      Rust_primitives.Hax.t_Never)
+assume
+val mm256_extracti128_si256':
+    v_CONTROL: i32 ->
+    vector: Minicore.Abstractions.Bitvec.t_BitVec (mk_u64 256)
+  -> Minicore.Abstractions.Bitvec.t_BitVec (mk_u64 128)
 
-let mm_movemask_epi8 (vector: Minicore.Abstractions.Bitvec.t_BitVec (mk_u64 128)) : i32 =
-  Rust_primitives.Hax.never_to_any (Core.Panicking.panic "not implemented"
-      <:
-      Rust_primitives.Hax.t_Never)
+let mm256_extracti128_si256 (v_CONTROL: i32) = mm256_extracti128_si256' v_CONTROL
+
+assume
+val mm256_inserti128_si256':
+    v_CONTROL: i32 ->
+    vector: Minicore.Abstractions.Bitvec.t_BitVec (mk_u64 256) ->
+    vector_i128: Minicore.Abstractions.Bitvec.t_BitVec (mk_u64 128)
+  -> Minicore.Abstractions.Bitvec.t_BitVec (mk_u64 256)
+
+let mm256_inserti128_si256 (v_CONTROL: i32) = mm256_inserti128_si256' v_CONTROL
+
+assume
+val mm256_blend_epi16':
+    v_CONTROL: i32 ->
+    lhs: Minicore.Abstractions.Bitvec.t_BitVec (mk_u64 256) ->
+    rhs: Minicore.Abstractions.Bitvec.t_BitVec (mk_u64 256)
+  -> Minicore.Abstractions.Bitvec.t_BitVec (mk_u64 256)
+
+let mm256_blend_epi16 (v_CONTROL: i32) = mm256_blend_epi16' v_CONTROL
+
+assume
+val mm256_blend_epi32':
+    v_CONTROL: i32 ->
+    lhs: Minicore.Abstractions.Bitvec.t_BitVec (mk_u64 256) ->
+    rhs: Minicore.Abstractions.Bitvec.t_BitVec (mk_u64 256)
+  -> Minicore.Abstractions.Bitvec.t_BitVec (mk_u64 256)
+
+let mm256_blend_epi32 (v_CONTROL: i32) = mm256_blend_epi32' v_CONTROL
+
+assume
+val vec256_blendv_epi32':
+    a: Minicore.Abstractions.Bitvec.t_BitVec (mk_u64 256) ->
+    b: Minicore.Abstractions.Bitvec.t_BitVec (mk_u64 256) ->
+    mask: Minicore.Abstractions.Bitvec.t_BitVec (mk_u64 256)
+  -> Minicore.Abstractions.Bitvec.t_BitVec (mk_u64 256)
+
+let vec256_blendv_epi32 = vec256_blendv_epi32'
+
+assume
+val mm_movemask_epi8': vector: Minicore.Abstractions.Bitvec.t_BitVec (mk_u64 128) -> i32
+
+let mm_movemask_epi8 = mm_movemask_epi8'
 
 let mm256_permutevar8x32_epi32 (vector control: Minicore.Abstractions.Bitvec.t_BitVec (mk_u64 256))
     : Minicore.Abstractions.Bitvec.t_BitVec (mk_u64 256) =
-  Rust_primitives.Hax.never_to_any (Core.Panicking.panic "not implemented"
-      <:
-      Rust_primitives.Hax.t_Never)
+  Minicore.Arch.X86.e_mm256_permutevar8x32_epi32 vector control
 
-let mm256_srlv_epi32 (vector counts: Minicore.Abstractions.Bitvec.t_BitVec (mk_u64 256))
-    : Minicore.Abstractions.Bitvec.t_BitVec (mk_u64 256) =
-  Rust_primitives.Hax.never_to_any (Core.Panicking.panic "not implemented"
-      <:
-      Rust_primitives.Hax.t_Never)
+assume
+val mm256_srlv_epi32':
+    vector: Minicore.Abstractions.Bitvec.t_BitVec (mk_u64 256) ->
+    counts: Minicore.Abstractions.Bitvec.t_BitVec (mk_u64 256)
+  -> Minicore.Abstractions.Bitvec.t_BitVec (mk_u64 256)
 
-let mm256_srlv_epi64 (vector counts: Minicore.Abstractions.Bitvec.t_BitVec (mk_u64 256))
-    : Minicore.Abstractions.Bitvec.t_BitVec (mk_u64 256) =
-  Rust_primitives.Hax.never_to_any (Core.Panicking.panic "not implemented"
-      <:
-      Rust_primitives.Hax.t_Never)
+let mm256_srlv_epi32 = mm256_srlv_epi32'
 
-let mm_sllv_epi32 (vector counts: Minicore.Abstractions.Bitvec.t_BitVec (mk_u64 128))
-    : Minicore.Abstractions.Bitvec.t_BitVec (mk_u64 128) =
-  Rust_primitives.Hax.never_to_any (Core.Panicking.panic "not implemented"
-      <:
-      Rust_primitives.Hax.t_Never)
+assume
+val mm256_srlv_epi64':
+    vector: Minicore.Abstractions.Bitvec.t_BitVec (mk_u64 256) ->
+    counts: Minicore.Abstractions.Bitvec.t_BitVec (mk_u64 256)
+  -> Minicore.Abstractions.Bitvec.t_BitVec (mk_u64 256)
+
+let mm256_srlv_epi64 = mm256_srlv_epi64'
+
+assume
+val mm_sllv_epi32':
+    vector: Minicore.Abstractions.Bitvec.t_BitVec (mk_u64 128) ->
+    counts: Minicore.Abstractions.Bitvec.t_BitVec (mk_u64 128)
+  -> Minicore.Abstractions.Bitvec.t_BitVec (mk_u64 128)
+
+let mm_sllv_epi32 = mm_sllv_epi32'
 
 let mm256_sllv_epi32 (vector counts: Minicore.Abstractions.Bitvec.t_BitVec (mk_u64 256))
     : Minicore.Abstractions.Bitvec.t_BitVec (mk_u64 256) =
-  Rust_primitives.Hax.never_to_any (Core.Panicking.panic "not implemented"
-      <:
-      Rust_primitives.Hax.t_Never)
+  Minicore.Arch.X86.e_mm256_sllv_epi32 vector counts
 
-let mm256_slli_epi64 (v_LEFT: i32) (x: Minicore.Abstractions.Bitvec.t_BitVec (mk_u64 256))
-    : Minicore.Abstractions.Bitvec.t_BitVec (mk_u64 256) =
-  Rust_primitives.Hax.never_to_any (Core.Panicking.panic "not implemented"
-      <:
-      Rust_primitives.Hax.t_Never)
+assume
+val mm256_slli_epi64': v_LEFT: i32 -> x: Minicore.Abstractions.Bitvec.t_BitVec (mk_u64 256)
+  -> Minicore.Abstractions.Bitvec.t_BitVec (mk_u64 256)
 
-let mm256_bsrli_epi128 (v_SHIFT_BY: i32) (x: Minicore.Abstractions.Bitvec.t_BitVec (mk_u64 256))
-    : Minicore.Abstractions.Bitvec.t_BitVec (mk_u64 256) =
-  let _:Prims.unit =
-    if true
-    then
-      let _:Prims.unit =
-        Hax_lib.v_assert ((v_SHIFT_BY >. mk_i32 0 <: bool) && (v_SHIFT_BY <. mk_i32 16 <: bool))
-      in
-      ()
-  in
-  Rust_primitives.Hax.never_to_any (Core.Panicking.panic "not implemented"
-      <:
-      Rust_primitives.Hax.t_Never)
+let mm256_slli_epi64 (v_LEFT: i32) = mm256_slli_epi64' v_LEFT
 
-let mm256_andnot_si256 (a b: Minicore.Abstractions.Bitvec.t_BitVec (mk_u64 256))
-    : Minicore.Abstractions.Bitvec.t_BitVec (mk_u64 256) =
-  Rust_primitives.Hax.never_to_any (Core.Panicking.panic "not implemented"
-      <:
-      Rust_primitives.Hax.t_Never)
+assume
+val mm256_bsrli_epi128': v_SHIFT_BY: i32 -> x: Minicore.Abstractions.Bitvec.t_BitVec (mk_u64 256)
+  -> Minicore.Abstractions.Bitvec.t_BitVec (mk_u64 256)
 
-let mm256_set1_epi64x (a: i64) : Minicore.Abstractions.Bitvec.t_BitVec (mk_u64 256) =
-  Rust_primitives.Hax.never_to_any (Core.Panicking.panic "not implemented"
-      <:
-      Rust_primitives.Hax.t_Never)
+let mm256_bsrli_epi128 (v_SHIFT_BY: i32) = mm256_bsrli_epi128' v_SHIFT_BY
 
-let mm256_set_epi64x (input3 input2 input1 input0: i64)
-    : Minicore.Abstractions.Bitvec.t_BitVec (mk_u64 256) =
-  Rust_primitives.Hax.never_to_any (Core.Panicking.panic "not implemented"
-      <:
-      Rust_primitives.Hax.t_Never)
+assume
+val mm256_andnot_si256':
+    a: Minicore.Abstractions.Bitvec.t_BitVec (mk_u64 256) ->
+    b: Minicore.Abstractions.Bitvec.t_BitVec (mk_u64 256)
+  -> Minicore.Abstractions.Bitvec.t_BitVec (mk_u64 256)
 
-let mm256_unpacklo_epi64 (a b: Minicore.Abstractions.Bitvec.t_BitVec (mk_u64 256))
-    : Minicore.Abstractions.Bitvec.t_BitVec (mk_u64 256) =
-  Rust_primitives.Hax.never_to_any (Core.Panicking.panic "not implemented"
-      <:
-      Rust_primitives.Hax.t_Never)
+let mm256_andnot_si256 = mm256_andnot_si256'
 
-let mm256_permute2x128_si256 (v_IMM8: i32) (a b: Minicore.Abstractions.Bitvec.t_BitVec (mk_u64 256))
-    : Minicore.Abstractions.Bitvec.t_BitVec (mk_u64 256) =
-  Rust_primitives.Hax.never_to_any (Core.Panicking.panic "not implemented"
-      <:
-      Rust_primitives.Hax.t_Never)
+assume
+val mm256_set1_epi64x': a: i64 -> Minicore.Abstractions.Bitvec.t_BitVec (mk_u64 256)
+
+let mm256_set1_epi64x = mm256_set1_epi64x'
+
+assume
+val mm256_set_epi64x': input3: i64 -> input2: i64 -> input1: i64 -> input0: i64
+  -> Minicore.Abstractions.Bitvec.t_BitVec (mk_u64 256)
+
+let mm256_set_epi64x = mm256_set_epi64x'
+
+assume
+val mm256_unpacklo_epi64':
+    a: Minicore.Abstractions.Bitvec.t_BitVec (mk_u64 256) ->
+    b: Minicore.Abstractions.Bitvec.t_BitVec (mk_u64 256)
+  -> Minicore.Abstractions.Bitvec.t_BitVec (mk_u64 256)
+
+let mm256_unpacklo_epi64 = mm256_unpacklo_epi64'
+
+assume
+val mm256_permute2x128_si256':
+    v_IMM8: i32 ->
+    a: Minicore.Abstractions.Bitvec.t_BitVec (mk_u64 256) ->
+    b: Minicore.Abstractions.Bitvec.t_BitVec (mk_u64 256)
+  -> Minicore.Abstractions.Bitvec.t_BitVec (mk_u64 256)
+
+let mm256_permute2x128_si256 (v_IMM8: i32) = mm256_permute2x128_si256' v_IMM8
